ocaml/extracted/extract.v
@@ -210,5 +210,6 @@ Separate Extraction
   traverse.traverse_pre'
   traverse.traverse_post
   traverse.list_rev_post
+  traverse.plain_blocks
   traverse.traverse_cps
 .
